fix layout in typing/type.v

theories/typing/type.v
@@ -64,11 +64,9 @@ Record type `{!typeG Σ} A := {
 }.
 Existing Instance ty_shr_persistent.
 
-Instance: Params (@ty_size) 3 := {}.
-Instance: Params (@ty_lfts) 3 := {}.
+Instance: Params (@ty_size) 3 := {}. Instance: Params (@ty_lfts) 3 := {}.
 Instance: Params (@ty_E) 3 := {}.
-Instance: Params (@ty_own) 3 := {}.
-Instance: Params (@ty_shr) 3 := {}.
+Instance: Params (@ty_own) 3 := {}. Instance: Params (@ty_shr) 3 := {}.
 
 Arguments ty_size {_ _ _} _ / : simpl nomatch.
 Arguments ty_lfts {_ _ _} _ / : simpl nomatch.
@@ -77,6 +75,7 @@ Arguments ty_own {_ _ _} _ _ _ _ / : simpl nomatch.
 Arguments ty_shr {_ _ _} _ _ _ _ _ / : simpl nomatch.
 
 Notation ty_lft ty := (lft_intersect_list ty.(ty_lfts)).
+Notation typel := (hlist type).
 
 Lemma ty_own_mt_depth_mono `{!typeG Σ} {A} (ty: _ A) d d' vπ tid l :
   d ≤ d' → l ↦∗: ty.(ty_own) (vπ,d) tid -∗ l ↦∗: ty.(ty_own) (vπ,d') tid.
@@ -89,8 +88,7 @@ Definition ty_outlives_E `{!typeG Σ} {A} (ty: _ A) (κ: lft) : elctx :=
   (λ α, κ ⊑ₑ α) <$> ty.(ty_lfts).
 
 Lemma ty_outlives_E_elctx_sat `{!typeG Σ} {A} E L (ty: _ A) α β :
-  ty_outlives_E ty β ⊆+ E →
-  lctx_lft_incl E L α β →
+  ty_outlives_E ty β ⊆+ E → lctx_lft_incl E L α β →
   elctx_sat E L (ty_outlives_E ty α).
 Proof.
   rewrite /ty_outlives_E. elim ty.(ty_lfts); [by solve_typing|].
@@ -111,14 +109,14 @@ Proof.
       [iApply lft_intersect_incl_l|iApply lft_intersect_incl_r].
 Qed.
 
-Definition tyl_lfts `{!typeG Σ} {As} (tyl: hlist type As) : list lft :=
+Definition tyl_lfts `{!typeG Σ} {As} (tyl: typel As) : list lft :=
   concat ((λ _, ty_lfts) +<$> tyl).
-Definition tyl_E `{!typeG Σ} {As} (tyl: hlist type As) : elctx :=
+Definition tyl_E `{!typeG Σ} {As} (tyl: typel As) : elctx :=
   concat ((λ _, ty_E) +<$> tyl).
-Definition tyl_outlives_E `{!typeG Σ} {As} (tyl: hlist type As) κ : elctx :=
+Definition tyl_outlives_E `{!typeG Σ} {As} (tyl: typel As) κ : elctx :=
   concat ((λ _ ty, ty_outlives_E ty κ) +<$> tyl).
 
-Lemma tyl_outlives_E_elctx_sat `{!typeG Σ} {As} E L (tyl: hlist type As) α β :
+Lemma tyl_outlives_E_elctx_sat `{!typeG Σ} {As} E L (tyl: typel As) α β :
   tyl_outlives_E tyl β ⊆+ E → lctx_lft_incl E L α β →
   elctx_sat E L (tyl_outlives_E tyl α).
 Proof.
@@ -147,20 +145,18 @@ Record simple_type `{!typeG Σ} A := {
       q':+[ξs] ∗ (q':+[ξs] ={E}=∗ st_own (vπ,d) tid vl ∗ q.[κ]);
 }.
 Existing Instance st_own_persistent.
-Instance: Params (@st_size) 3 := {}.
-Instance: Params (@st_lfts) 3 := {}.
-Instance: Params (@st_E) 3 := {}.
-Instance: Params (@st_own) 3 := {}.
+Instance: Params (@st_size) 3 := {}. Instance: Params (@st_lfts) 3 := {}.
+Instance: Params (@st_E) 3 := {}. Instance: Params (@st_own) 3 := {}.
 Arguments st_size {_ _ _} _ / : simpl nomatch.
 Arguments st_lfts {_ _ _} _ / : simpl nomatch.
 Arguments st_E {_ _ _} _ / : simpl nomatch.
 Arguments st_own {_ _ _} _ _ _ _ / : simpl nomatch.
 
-Program Definition ty_of_st `{!typeG Σ} {A} (st: simple_type A) : type A :=
-  {| ty_size := st.(st_size);  ty_lfts := st.(st_lfts);  ty_E := st.(st_E);
-     ty_own := st.(st_own);
-     ty_shr vπd κ tid l := (∃vl,
-       &frac{κ} (λ q, l ↦∗{q} vl) ∗ ▷ st.(st_own) vπd tid vl)%I |}.
+Program Definition ty_of_st `{!typeG Σ} {A} (st: simple_type A) : type A := {|
+  ty_size := st.(st_size);  ty_lfts := st.(st_lfts);  ty_E := st.(st_E);
+  ty_own := st.(st_own);
+  ty_shr vπd κ tid l := (∃vl, &frac{κ} (λ q, l ↦∗{q} vl) ∗ ▷ st.(st_own) vπd tid vl)%I;
+|}.
 Next Obligation. move=> >. apply st_size_eq. Qed.
 Next Obligation. move=> >. by apply st_own_depth_mono. Qed.
 Next Obligation.
@@ -176,14 +172,12 @@ Next Obligation.
   iMod (bor_exists with "LFT Bor") as (vl) "Bor"; [done|].
   iMod (bor_sep with "LFT Bor") as "[Bor Own]"; [done|].
   iMod (bor_persistent with "LFT Own Tok") as "[??]"; [done|].
-  iMod (bor_fracture (λ q, _ ↦∗{q} vl)%I with "LFT Bor") as "?"; [done|].
-  iModIntro. iApply step_fupdN_intro; [done|]. iNext. iModIntro. iFrame.
-  iExists vl. iFrame.
+  iMod (bor_fracture (λ q, _ ↦∗{q} vl)%I with "LFT Bor") as "?"; [done|]. iModIntro.
+  iApply step_fupdN_intro; [done|]. iNext. iModIntro. iFrame. iExists vl. iFrame.
 Qed.
 Next Obligation. move=> >. apply st_own_proph. Qed.
 Next Obligation.
-  move=> *. iIntros "#LFT _ Incl". iDestruct 1 as (vl) "[? Own]".
-  iIntros "Tok !>!>".
+  move=> *. iIntros "#LFT _ Incl". iDestruct 1 as (vl) "[? Own]". iIntros "Tok !>!>".
   iDestruct (st_own_proph with "LFT Incl Own Tok") as "> Upd"; [done|].
   iModIntro. iApply (step_fupdN_wand with "Upd"). iDestruct 1 as "> Upd".
   iDestruct "Upd" as (ξs q' ?) "[Ptoks Upd]". iModIntro. iExists ξs, q'.
@@ -202,18 +196,17 @@ Record plain_type `{!typeG Σ} A := {
   pt_size_eq v tid vl : pt_own v tid vl -∗ ⌜length vl = pt_size⌝;
 }.
 Existing Instance pt_own_persistent.
-Instance: Params (@pt_size) 3 := {}.
-Instance: Params (@pt_lfts) 3 := {}.
-Instance: Params (@pt_E) 3 := {}.
-Instance: Params (@pt_own) 3 := {}.
+Instance: Params (@pt_size) 3 := {}. Instance: Params (@pt_lfts) 3 := {}.
+Instance: Params (@pt_E) 3 := {}. Instance: Params (@pt_own) 3 := {}.
 Arguments pt_size {_ _ _} _ / : simpl nomatch.
 Arguments pt_lfts {_ _ _} _ / : simpl nomatch.
 Arguments pt_E {_ _ _} _ / : simpl nomatch.
 Arguments pt_own {_ _ _} _ _ _ _ / : simpl nomatch.
 
-Program Definition st_of_pt `{!typeG Σ} {A} (pt: plain_type A) : simple_type A :=
-  {| st_size := pt.(pt_size);  st_lfts := pt.(pt_lfts);  st_E := pt.(pt_E);
-     st_own vπd tid vl := (∃v, ⌜vπd.1 = const v⌝ ∗ pt.(pt_own) v tid vl)%I |}.
+Program Definition st_of_pt `{!typeG Σ} {A} (pt: plain_type A) : simple_type A := {|
+  st_size := pt.(pt_size);  st_lfts := pt.(pt_lfts);  st_E := pt.(pt_E);
+  st_own vπd tid vl := (∃v, ⌜vπd.1 = const v⌝ ∗ pt.(pt_own) v tid vl)%I;
+|}.
 Next Obligation. move=> >. iDestruct 1 as (? _) "?". by iApply pt_size_eq. Qed.
 Next Obligation. done. Qed.
 Next Obligation.
@@ -256,7 +249,7 @@ Section ofe.
   Definition type_ofe_mixin {A} : OfeMixin (type A).
   Proof.
     apply (iso_ofe_mixin type_unpack);
-    (rewrite /type_unpack; split; [by move=> [-> -> -> ??]|]);
+    (rewrite /type_unpack; split; [by move=> [->->->??]|]);
     move=> [[[[??]?]?]?]; simpl in *; constructor; try apply leibniz_equiv;
     try done; by eapply (discrete_iff _ _).
   Qed.
@@ -281,35 +274,35 @@ Section ofe.
     Proper ((≡) ==> (=) ==> (=)) (@ty_outlives_E _ _ A).
   Proof. rewrite /ty_outlives_E. by move=> ?? [_ -> _ _ _]. Qed.
 
-  Global Instance hlist_dist_type {As} : Dist (hlist type As) := @hlist_dist (@typeO) _.
+  Global Instance hlist_dist_type {As} : Dist (typel As) := @hlist_dist (@typeO) _.
 
   Global Instance tyl_E_ne {As} n : Proper (dist n ==> (=)) (@tyl_E _ _ As).
-  Proof. move=> ??. rewrite /tyl_E. by elim=> [|/= > -> _ ->]. Qed.
+  Proof. move=> ??. rewrite /tyl_E. by elim=> /=[|> ->_->]. Qed.
   Global Instance tyl_E_proper {As} : Proper ((≡) ==> (=)) (@tyl_E _ _ As).
-  Proof. move=> ??. rewrite /tyl_E. by elim=> [|/= > -> _ ->]. Qed.
+  Proof. move=> ??. rewrite /tyl_E. by elim=> /=[|> ->_->]. Qed.
   Global Instance tyl_outlives_E_ne {As} n :
     Proper (dist n ==> (=) ==> (=)) (@tyl_outlives_E _ _ As).
   Proof.
-    move=> ?? Eqv ??->. rewrite /tyl_outlives_E. by elim Eqv=> [|/= > -> _ ->].
+    move=> ?? Eqv ??->. rewrite /tyl_outlives_E. by elim Eqv=> /=[|> ->_->].
   Qed.
   Global Instance tyl_outlives_E_proper {A} :
     Proper ((≡) ==> (=) ==> (=)) (@tyl_outlives_E _ _ A).
   Proof.
-    move=> ?? Eqv ??->. rewrite /tyl_outlives_E. by elim Eqv=> [|/= > -> _ ->].
+    move=> ?? Eqv ??->. rewrite /tyl_outlives_E. by elim Eqv=> /=[|> ->_->].
   Qed.
 
   Global Instance ty_own_ne {A} n:
     Proper (dist n ==> (=) ==> (=) ==> (=) ==> dist n) (@ty_own _ _ A).
-  Proof. move=> ?? Eqv ??-> ??-> ??->. apply Eqv. Qed.
+  Proof. move=> ?? Eqv ??->??->??->. apply Eqv. Qed.
   Global Instance ty_own_proper {A} :
     Proper ((≡) ==> (=) ==> (=) ==> (=) ==> (≡)) (@ty_own _ _ A).
-  Proof. move=> ?? Eqv ??-> ??-> ??->. apply Eqv. Qed.
+  Proof. move=> ?? Eqv ??->??->??->. apply Eqv. Qed.
   Global Instance ty_shr_ne {A} n :
     Proper (dist n ==> (=) ==> (=) ==> (=) ==> (=) ==> dist n) (@ty_shr _ _ A).
-  Proof. move=> ?? Eqv ??-> ??-> ??-> ??->. apply Eqv. Qed.
+  Proof. move=> ?? Eqv ??->??->??->??->. apply Eqv. Qed.
   Global Instance ty_shr_proper {A} :
     Proper ((≡) ==> (=) ==> (=) ==> (=) ==> (=) ==> (≡)) (@ty_shr _ _ A).
-  Proof. move=> ?? Eqv ??-> ??-> ??-> ??->. apply Eqv. Qed.
+  Proof. move=> ?? Eqv ??->??->??->??->. apply Eqv. Qed.
 
   (** Simple Type *)
 
@@ -336,10 +329,10 @@ Section ofe.
 
   Global Instance st_own_ne n {A} :
     Proper (dist n ==> (=) ==> (=) ==> (=) ==> dist n) (@st_own _ _ A).
-  Proof. move=> ?? Eqv ??-> ??-> ??->. apply Eqv. Qed.
+  Proof. move=> ?? Eqv ??->??->??->. apply Eqv. Qed.
   Global Instance st_own_proper {A} :
     Proper ((≡) ==> (=) ==> (=) ==> (=) ==> (≡)) (@st_own _ _ A).
-  Proof. move=> ?? Eqv ??-> ??-> ??->. apply Eqv. Qed.
+  Proof. move=> ?? Eqv ??->??->??->. apply Eqv. Qed.
 
   Global Instance ty_of_st_ne {A} : NonExpansive (@ty_of_st _ _ A).
   Proof.
@@ -373,7 +366,7 @@ Section ofe.
   Definition plain_type_ofe_mixin {A} : OfeMixin (plain_type A).
   Proof.
     apply (iso_ofe_mixin plain_type_unpack);
-    (rewrite /plain_type_unpack; split; [by move=> [-> -> -> ?]|]);
+    (rewrite /plain_type_unpack; split; [by move=> [->->->?]|]);
     move=> [[[??]?]?]; simpl in *; constructor; try apply leibniz_equiv;
     try done; by eapply (discrete_iff _ _).
   Qed.
@@ -381,10 +374,10 @@ Section ofe.
 
   Global Instance pt_own_ne n {A} :
     Proper (dist n ==> (=) ==> (=) ==> (=) ==> dist n) (@pt_own _ _ A).
-  Proof. move=> ?? Eqv ??-> ??-> ??->. apply Eqv. Qed.
+  Proof. move=> ?? Eqv ??->??->??->. apply Eqv. Qed.
   Global Instance pt_own_proper {A} :
     Proper ((≡) ==> (=) ==> (=) ==> (=) ==> (≡)) (@pt_own _ _ A).
-  Proof. move=> ?? Eqv ??-> ??-> ??->. apply Eqv. Qed.
+  Proof. move=> ?? Eqv ??->??->??->. apply Eqv. Qed.
 
   Global Instance st_of_pt_ne {A} : NonExpansive (@st_of_pt _ _ A).
   Proof.
@@ -407,8 +400,8 @@ Ltac solve_ne_type :=
 Inductive TypeLftMorphism `{!typeG Σ} {A B} (T : type A → type B) : Prop :=
 | type_lft_morphism_add α βs E :
     (∀ty, ⊢ (T ty).(ty_lft) ≡ₗ α ⊓ ty.(ty_lft)) →
-    (∀ty, elctx_interp (T ty).(ty_E) ⊣⊢ elctx_interp E ∗
-            elctx_interp ty.(ty_E) ∗ [∗ list] β ∈ βs, β ⊑ ty.(ty_lft)) →
+    (∀ty, elctx_interp (T ty).(ty_E) ⊣⊢
+      elctx_interp E ∗ elctx_interp ty.(ty_E) ∗ [∗ list] β ∈ βs, β ⊑ ty.(ty_lft)) →
     TypeLftMorphism T
 | type_lft_morphism_const α E :
     (∀ty, ⊢ (T ty).(ty_lft) ≡ₗ α) →
@@ -419,7 +412,7 @@ Existing Class TypeLftMorphism.
 Section type_lft_morphism.
 Context `{!typeG Σ}.
 
-Global Instance type_lft_morphism_compose {A B C} (T: _ B → _ C) (U: _ A → _ B):
+Global Instance type_lft_morphism_compose {A B C} (T: _ B → _ C) (U: _ A → _ B) :
   TypeLftMorphism T → TypeLftMorphism U → TypeLftMorphism (T ∘ U).
 Proof.
   destruct 1 as [αT βsT ET HTα HTE|αT ET HTα HTE],
@@ -462,13 +455,11 @@ Qed.
 
 Lemma type_lft_morphism_elctx_interp_proper {A B} (T: _ A → _ B)
   {HT: TypeLftMorphism T} ty1 ty2 :
-  elctx_interp ty1.(ty_E) ≡ elctx_interp ty2.(ty_E) →
-  (⊢ ty1.(ty_lft) ≡ₗ ty2.(ty_lft)) →
+  elctx_interp ty1.(ty_E) ≡ elctx_interp ty2.(ty_E) → (⊢ ty1.(ty_lft) ≡ₗ ty2.(ty_lft)) →
   elctx_interp (T ty1).(ty_E) ≡ elctx_interp (T ty2).(ty_E).
 Proof.
-  intros HE12 Hl. destruct HT as [α βs E Hα HE|α E Hα HE].
-  - rewrite !HE HE12. do 5 f_equiv. by apply lft_incl_equiv_proper_r.
-  - by rewrite !HE.
+  intros HE12 Hl. destruct HT as [α βs E Hα HE|α E Hα HE]; [|by rewrite !HE].
+  rewrite !HE HE12. do 5 f_equiv. by apply lft_incl_equiv_proper_r.
 Qed.
 
 Lemma type_lft_morphism_ext {A B} (T U: _ A → _ B) :
@@ -477,34 +468,28 @@ Proof. by intros [] HTU; [eleft|eright]; intros; rewrite -HTU. Qed.
 
 End type_lft_morphism.
 
-Class TypeContractive `{!typeG Σ} {A B} (T: type A -> type B): Prop := {
+Class TypeContractive `{!typeG Σ} {A B} (T: type A -> type B) : Prop := {
   type_contractive_type_lft_morphism : TypeLftMorphism T;
 
   type_contractive_ty_size ty1 ty2 : (T ty1).(ty_size) = (T ty2).(ty_size);
 
   type_contractive_ty_own n ty1 ty2 :
-    ty1.(ty_size) = ty2.(ty_size) →
-    (⊢ ty1.(ty_lft) ≡ₗ ty2.(ty_lft)) →
+    ty1.(ty_size) = ty2.(ty_size) → (⊢ ty1.(ty_lft) ≡ₗ ty2.(ty_lft)) →
     elctx_interp (ty1.(ty_E)) ≡ elctx_interp (ty2.(ty_E)) →
-    (∀vπd tid vl,
-      dist_later n (ty1.(ty_own) vπd tid vl) (ty2.(ty_own) vπd tid vl)) →
+    (∀vπd tid vl, dist_later n (ty1.(ty_own) vπd tid vl) (ty2.(ty_own) vπd tid vl)) →
     (∀vπd κ tid l, ty1.(ty_shr) vπd κ tid l ≡{n}≡ ty2.(ty_shr) vπd κ tid l) →
-    (∀vπd tid vl,
-      (T ty1).(ty_own) vπd tid vl ≡{n}≡ (T ty2).(ty_own) vπd tid vl);
+    (∀vπd tid vl, (T ty1).(ty_own) vπd tid vl ≡{n}≡ (T ty2).(ty_own) vπd tid vl);
 
   type_contractive_ty_shr n ty1 ty2 :
-    ty1.(ty_size) = ty2.(ty_size) →
-    (⊢ ty1.(ty_lft) ≡ₗ ty2.(ty_lft)) →
+    ty1.(ty_size) = ty2.(ty_size) → (⊢ ty1.(ty_lft) ≡ₗ ty2.(ty_lft)) →
     elctx_interp (ty1.(ty_E)) ≡ elctx_interp (ty2.(ty_E)) →
     (∀vπd tid vl, match n with S (S n) =>
       ty1.(ty_own) vπd tid vl ≡{n}≡ ty2.(ty_own) vπd tid vl | _ => True end) →
-    (∀vπd κ tid l,
-      dist_later n (ty1.(ty_shr) vπd κ tid l) (ty2.(ty_shr) vπd κ tid l)) →
-    (∀vπd κ tid l,
-      (T ty1).(ty_shr) vπd κ tid l ≡{n}≡ (T ty2).(ty_shr) vπd κ tid l);
+    (∀vπd κ tid l, dist_later n (ty1.(ty_shr) vπd κ tid l) (ty2.(ty_shr) vπd κ tid l)) →
+    (∀vπd κ tid l, (T ty1).(ty_shr) vπd κ tid l ≡{n}≡ (T ty2).(ty_shr) vπd κ tid l);
 }.
 
-Class TypeNonExpansive `{!typeG Σ} {A B} (T : type A -> type B): Prop := {
+Class TypeNonExpansive `{!typeG Σ} {A B} (T : type A -> type B) : Prop := {
   type_non_expansive_type_lft_morphism :> TypeLftMorphism T;
 
   type_non_expansive_ty_size ty1 ty2 :
@@ -530,13 +515,13 @@ Class TypeNonExpansive `{!typeG Σ} {A B} (T : type A -> type B): Prop := {
       (T ty1).(ty_shr) vπd κ tid l ≡{n}≡ (T ty2).(ty_shr) vπd κ tid l);
 }.
 
-Class TypeListNonExpansive `{!typeG Σ} {A Bs} (T: type A → hlist type Bs) : Prop
-:= type_list_non_expansive: ∃Tl,
+Class TypeListNonExpansive `{!typeG Σ} {A Bs} (T: type A → typel Bs) : Prop :=
+  type_list_non_expansive: ∃Tl,
     (∀ty, T ty = (λ B (T': type A → type B), T' ty) +<$>+ Tl) ∧
     HForall (λ _, TypeNonExpansive) Tl.
 
-Class TypeListContractive `{!typeG Σ} {A Bs} (T: type A → hlist type Bs) : Prop
-:= type_list_contractive: ∃Tl,
+Class TypeListContractive `{!typeG Σ} {A Bs} (T: type A → typel Bs) : Prop :=
+  type_list_contractive: ∃Tl,
     (∀ty, T ty = (λ B (T': type A → type B), T' ty) +<$>+ Tl) ∧
     HForall (λ _, TypeContractive) Tl.
 
@@ -610,28 +595,23 @@ Section type_contractive.
       + apply type_lft_morphism_elctx_interp_proper=>//. apply _.
   Qed.
 
-  Global Instance const_type_contractive {A B} (ty: _ B) :
-    TypeContractive (λ (_: _ A), ty).
+  Global Instance const_type_contractive {A B} (ty: _ B) : TypeContractive (λ _: _ A, ty).
   Proof. split; intros=>//. eright=>_. iApply lft_equiv_refl. done. Qed.
 
-  Global Instance id_type_non_expansive {A} :
-    TypeNonExpansive (id: _ A → _ A).
+  Global Instance id_type_non_expansive {A} : TypeNonExpansive (id: _ A → _ A).
   Proof.
     split; intros=>//. apply (type_lft_morphism_add _ static [] []).
     - intros. rewrite left_id. apply lft_equiv_refl.
     - intros. by rewrite /elctx_interp /= left_id right_id.
   Qed.
 
-  Global Instance type_list_non_expansive_nil {A} :
-    TypeListNonExpansive (λ (_: _ A), +[]).
+  Global Instance type_list_non_expansive_nil {A} : TypeListNonExpansive (λ _: _ A, +[]).
   Proof. exists +[]. split; by [|constructor]. Qed.
 
-  Global Instance type_list_contractive_nil {A} :
-    TypeListContractive (λ (_: _ A), +[]).
+  Global Instance type_list_contractive_nil {A} : TypeListContractive (λ _: _ A, +[]).
   Proof. exists +[]. split; by [|constructor]. Qed.
 
-  Global Instance type_list_non_expansive_cons {A B Bs}
-    (T: _ A → _ B) (Tl: _ A → _ Bs) :
+  Global Instance type_list_non_expansive_cons {A B Bs} (T: _ A → _ B) (Tl: _ A → _ Bs) :
     TypeNonExpansive T → TypeListNonExpansive Tl →
     TypeListNonExpansive (λ ty, T ty +:: Tl ty).
   Proof.
@@ -639,8 +619,7 @@ Section type_contractive.
     by rewrite Eq.
   Qed.
 
-  Global Instance type_list_contractive_cons {A B Bs}
-    (T: _ A → _ B) (Tl: _ A → _ Bs) :
+  Global Instance type_list_contractive_cons {A B Bs} (T: _ A → _ B) (Tl: _ A → _ Bs) :
     TypeContractive T → TypeListContractive Tl →
     TypeListContractive (λ ty, T ty +:: Tl ty).
   Proof.
@@ -653,26 +632,22 @@ End type_contractive.
 (** * Traits *)
 
 Fixpoint shr_locsE (l: loc) (n: nat) : coPset :=
-  match n with
-  | 0%nat => ∅
-  | S n => ↑shrN.@l ∪ shr_locsE (l +ₗ 1%nat) n
-  end.
+  match n with 0%nat => ∅ | S n => ↑shrN.@l ∪ shr_locsE (l +ₗ 1%nat) n end.
 
 Class Copy `{!typeG Σ} {A} (ty: type A) := {
   copy_persistent vπd tid vl : Persistent (ty.(ty_own) vπd tid vl);
   copy_shr_acc vπd κ tid E F l q :
     ↑lftN ∪ ↑shrN ⊆ E → shr_locsE l (ty.(ty_size) + 1) ⊆ F →
-    lft_ctx -∗ ty.(ty_shr) vπd κ tid l -∗ na_own tid F -∗ q.[κ] ={E}=∗
-       ∃ q' vl, na_own tid (F ∖ shr_locsE l ty.(ty_size)) ∗
-         l ↦∗{q'} vl ∗ ▷ty.(ty_own) vπd tid vl ∗
+    lft_ctx -∗ ty.(ty_shr) vπd κ tid l -∗ na_own tid F -∗ q.[κ] ={E}=∗ ∃q' vl,
+      na_own tid (F ∖ shr_locsE l ty.(ty_size)) ∗
+      l ↦∗{q'} vl ∗ ▷ty.(ty_own) vπd tid vl ∗
       (na_own tid (F ∖ shr_locsE l ty.(ty_size)) -∗ l ↦∗{q'} vl
-       ={E}=∗ na_own tid F ∗ q.[κ])
+        ={E}=∗ na_own tid F ∗ q.[κ])
 }.
 Existing Instances copy_persistent.
 Instance: Params (@Copy) 3 := {}.
 
-Class ListCopy `{!typeG Σ} {As} (tyl: hlist type As) :=
-  list_copy: HForall (λ _, Copy) tyl.
+Class ListCopy `{!typeG Σ} {As} (tyl: typel As) := list_copy: HForall (λ _, Copy) tyl.
 Instance: Params (@ListCopy) 3 := {}.
 Global Instance list_copy_nil `{!typeG Σ} : ListCopy +[].
 Proof. constructor. Qed.
@@ -685,8 +660,7 @@ Class Send `{!typeG Σ} {A} (ty: type A) :=
     ty.(ty_own) vπd tid1 vl -∗ ty.(ty_own) vπd tid2 vl.
 Instance: Params (@Send) 3 := {}.
 
-Class ListSend `{!typeG Σ} {As} (tyl: hlist type As) :=
-  list_send : HForall (λ _, Send) tyl.
+Class ListSend `{!typeG Σ} {As} (tyl: typel As) := list_send: HForall (λ _, Send) tyl.
 Instance: Params (@ListSend) 3 := {}.
 Global Instance list_send_nil `{!typeG Σ} : ListSend +[].
 Proof. constructor. Qed.
@@ -699,8 +673,7 @@ Class Sync `{!typeG Σ} {A} (ty: type A) :=
     ty.(ty_shr) vπd κ tid1 l -∗ ty.(ty_shr) vπd κ tid2 l.
 Instance: Params (@Sync) 3 := {}.
 
-Class ListSync `{!typeG Σ} {As} (tyl: hlist type As) :=
-  list_sync : HForall (λ _, Sync) tyl.
+Class ListSync `{!typeG Σ} {As} (tyl: typel As) := list_sync : HForall (λ _, Sync) tyl.
 Instance: Params (@ListSync) 3 := {}.
 Global Instance list_sync_nil `{!typeG Σ} : ListSync +[].
 Proof. constructor. Qed.
@@ -751,7 +724,7 @@ Section type.
 
   Lemma shr_locsE_split_tok l n m tid :
     na_own tid (shr_locsE l (n + m)) ⊣⊢
-      na_own tid (shr_locsE l n) ∗ na_own tid (shr_locsE (l +ₗ n) m).
+    na_own tid (shr_locsE l n) ∗ na_own tid (shr_locsE (l +ₗ n) m).
   Proof.
     rewrite shr_locsE_shift na_own_union //. apply shr_locsE_disj.
   Qed.
@@ -769,8 +742,7 @@ Section type.
     move=> *. iIntros "#LFT #Hshr Htok Hlft /=".
     iDestruct (na_own_acc with "Htok") as "[$ Htok]"; [solve_ndisj|].
     iDestruct "Hshr" as (vl) "[Hf Hown]".
-    iMod (frac_bor_acc with "LFT Hf Hlft") as (q') "[>Hmt Hclose]";
-      [solve_ndisj|].
+    iMod (frac_bor_acc with "LFT Hf Hlft") as (q') "[>Hmt Hclose]"; [solve_ndisj|].
     iModIntro. iExists _, _. iFrame "Hmt Hown". iIntros "Htok2".
     iDestruct ("Htok" with "Htok2") as "$". iIntros "Hmt". by iApply "Hclose".
   Qed.
@@ -778,17 +750,12 @@ Section type.
   (** Lemmas on Send and Sync *)
 
   Global Instance send_equiv {A} : Proper (equiv ==> impl) (@Send _ _ A).
-  Proof.
-    move=> ?? [_ _ _ Eqv _] ?. rewrite /Send=> *. by rewrite -!Eqv.
-  Qed.
+  Proof. move=> ?? [_ _ _ Eqv _] ?. rewrite /Send=> *. by rewrite -!Eqv. Qed.
 
   Global Instance sync_equiv {A} : Proper (equiv ==> impl) (@Sync _ _ A).
-  Proof.
-    move=> ?? [_ _ _ _ Eqv] ?. rewrite /Sync=> *. by rewrite -!Eqv.
-  Qed.
+  Proof. move=> ?? [_ _ _ _ Eqv] ?. rewrite /Sync=> *. by rewrite -!Eqv. Qed.
 
-  Global Instance ty_of_st_sync {A} (st: _ A) :
-    Send (ty_of_st st) → Sync (ty_of_st st).
+  Global Instance ty_of_st_sync {A} (st: _ A) : Send (ty_of_st st) → Sync (ty_of_st st).
   Proof.
     move=> Hsend >. iDestruct 1 as (vl) "[Hm Hown]".
     iExists vl. iFrame "Hm". iNext. by iApply Hsend.
@@ -796,27 +763,22 @@ Section type.
 
   Lemma send_change_tid' {A} (ty: _ A) vπd tid1 tid2 vl :
     Send ty → ty.(ty_own) vπd tid1 vl ≡ ty.(ty_own) vπd tid2 vl.
-  Proof.
-    intros ?. apply: anti_symm; apply send_change_tid.
-  Qed.
+  Proof. move=> ?. apply: anti_symm; apply send_change_tid. Qed.
 
   Lemma sync_change_tid' {A} (ty: _ A) vπd κ tid1 tid2 l :
     Sync ty → ty.(ty_shr) vπd κ tid1 l ≡ ty.(ty_shr) vπd κ tid2 l.
-  Proof.
-    intros ?. apply: anti_symm; apply sync_change_tid.
-  Qed.
+  Proof. move=> ?. apply: anti_symm; apply sync_change_tid. Qed.
 
 End type.
 
 (** * Subtyping *)
 
 Definition type_incl `{!typeG Σ} {A B} (f: A → B) ty1 ty2 : iProp Σ :=
-  ⌜ty1.(ty_size) = ty2.(ty_size)⌝ ∗
-  (ty2.(ty_lft) ⊑ ty1.(ty_lft)) ∗
+  ⌜ty1.(ty_size) = ty2.(ty_size)⌝ ∗ (ty2.(ty_lft) ⊑ ty1.(ty_lft)) ∗
   (□ ∀vπ d tid vl,
-    ty1.(ty_own) (vπ, d) tid vl -∗ ty2.(ty_own) (f ∘ vπ, d) tid vl) ∗
+    ty1.(ty_own) (vπ,d) tid vl -∗ ty2.(ty_own) (f∘vπ,d) tid vl) ∗
   (□ ∀vπ d κ tid l,
-    ty1.(ty_shr) (vπ, d) κ tid l -∗ ty2.(ty_shr) (f ∘ vπ, d) κ tid l).
+    ty1.(ty_shr) (vπ,d) κ tid l -∗ ty2.(ty_shr) (f∘vπ,d) κ tid l).
 Instance: Params (@type_incl) 4 := {}.
 
 Definition subtype `{!typeG Σ} {A B} E L (f: A → B) ty1 ty2 : Prop :=
@@ -912,10 +874,8 @@ Section subtyping.
     ∀qL, llctx_interp L qL -∗ □ (elctx_interp E -∗
       ⌜ty1.(ty_size) = ty2.(ty_size)⌝ ∗
       (ty1.(ty_lft) ≡ₗ ty2.(ty_lft)) ∗
-      (□ ∀vπ d tid vl,
-        ty1.(ty_own) (vπ, d) tid vl ↔ ty2.(ty_own) (f ∘ vπ, d) tid vl) ∗
-      (□ ∀vπ d κ tid l,
-        ty1.(ty_shr) (vπ, d) κ tid l ↔ ty2.(ty_shr) (f ∘ vπ, d) κ tid l)).
+      (□ ∀vπ d tid vl, ty1.(ty_own) (vπ,d) tid vl ↔ ty2.(ty_own) (f∘vπ,d) tid vl) ∗
+      (□ ∀vπ d κ tid l, ty1.(ty_shr) (vπ,d) κ tid l ↔ ty2.(ty_shr) (f∘vπ,d) κ tid l)).
   Proof.
     move=> Eq_gf Eq_fg. split.
     - iIntros ([EQ1 EQ2] qL) "HL".
@@ -931,8 +891,8 @@ Section subtyping.
       iDestruct (EQ with "HL") as "#EQ"; iIntros "!> #HE";
       iDestruct ("EQ" with "HE") as "(% & [??] & #Ho & #Hs)";
       (iSplit; [done|]; iSplit; [done|]; iSplit); iIntros "!> * Own";
-      [by iApply "Ho"|by iApply "Hs"| |];
-      [iApply "Ho"|iApply "Hs"]; by rewrite compose_assoc Eq_fg.
+      [by iApply "Ho"|by iApply "Hs"| |]; [iApply "Ho"|iApply "Hs"];
+      by rewrite compose_assoc Eq_fg.
   Qed.
 
   Lemma eqtype_refl {A} E L (ty: _ A) : eqtype E L id id ty ty.
@@ -966,8 +926,7 @@ Section subtyping.
 
   Lemma type_incl_simple_type {A B} f (st1: simple_type A) (st2: simple_type B) :
     st1.(st_size) = st2.(st_size) → st2.(ty_lft) ⊑ st1.(ty_lft) -∗
-    □ (∀vπ d tid vl,
-      st1.(st_own) (vπ, d) tid vl -∗ st2.(st_own) (f ∘ vπ, d) tid vl) -∗
+    □ (∀vπ d tid vl, st1.(st_own) (vπ,d) tid vl -∗ st2.(st_own) (f∘vπ,d) tid vl) -∗
     type_incl f st1 st2.
   Proof.
     move=> ?. iIntros "#Hl #Ho". iSplit; [done|]. iSplit; [done|].
@@ -980,8 +939,7 @@ Section subtyping.
   Lemma subtype_simple_type {A B} E L f (st1: simple_type A) (st2: simple_type B) :
     (∀qL, llctx_interp L qL -∗ □ (elctx_interp E -∗
       ⌜st1.(st_size) = st2.(st_size)⌝ ∗ st2.(ty_lft) ⊑ st1.(ty_lft) ∗
-      (∀vπ d tid vl,
-        st1.(st_own) (vπ, d) tid vl -∗ st2.(st_own) (f ∘ vπ, d) tid vl))) →
+      (∀vπ d tid vl, st1.(st_own) (vπ,d) tid vl -∗ st2.(st_own) (f∘vπ,d) tid vl))) →
     subtype E L f st1 st2.
   Proof.
     intros Hst. iIntros (qL) "HL". iDestruct (Hst with "HL") as "#Hst".
@@ -993,8 +951,7 @@ Section subtyping.
 
   Lemma type_incl_plain_type {A B} f (pt1: plain_type A) (pt2: plain_type B) :
     pt1.(pt_size) = pt2.(pt_size) → pt2.(ty_lft) ⊑ pt1.(ty_lft) -∗
-    □ (∀v tid vl,
-      pt1.(pt_own) v tid vl -∗ pt2.(pt_own) (f v) tid vl) -∗
+    □ (∀v tid vl, pt1.(pt_own) v tid vl -∗ pt2.(pt_own) (f v) tid vl) -∗
     type_incl f pt1 pt2.
   Proof.
     move=> ?. iIntros "#Hl #Ho". iSplit; [done|]. iSplit; [done|].
@@ -1008,8 +965,7 @@ Section subtyping.
   Lemma subtype_plain_type {A B} E L f (pt1: plain_type A) (pt2: plain_type B) :
     (∀qL, llctx_interp L qL -∗ □ (elctx_interp E -∗
       ⌜pt1.(pt_size) = pt2.(pt_size)⌝ ∗ pt2.(ty_lft) ⊑ pt1.(ty_lft) ∗
-      (∀v tid vl,
-        pt1.(pt_own) v tid vl -∗ pt2.(pt_own) (f v) tid vl))) →
+      (∀v tid vl, pt1.(pt_own) v tid vl -∗ pt2.(pt_own) (f v) tid vl))) →
     subtype E L f pt1 pt2.
   Proof.
     intros Hst. iIntros (qL) "HL". iDestruct (Hst with "HL") as "#Hst".
@@ -1034,7 +990,6 @@ Section type_util.
   Qed.
 End type_util.
 
-Global Hint Resolve ty_outlives_E_elctx_sat tyl_outlives_E_elctx_sat
-  : lrust_typing.
+Global Hint Resolve ty_outlives_E_elctx_sat tyl_outlives_E_elctx_sat : lrust_typing.
 Global Hint Resolve subtype_refl eqtype_refl : lrust_typing.
 Global Hint Opaque subtype eqtype : lrust_typing.
